remove extra parameters

frodo/code/Hacl.Impl.Frodo.KEM.Encaps.fst
@@ -278,7 +278,7 @@ val crypto_kem_enc_ct_inner:
       disjoint seed_a ct /\ disjoint seed_e ct /\ disjoint sp_matrix ct)
     (ensures fun h0 _ h1 -> modifies (loc_buffer ct) h0 h1 /\
        as_seq h1 ct == S.crypto_kem_enc_ct_inner (as_seq h0 seed_a) (as_seq h0 seed_e) (as_seq h0 b)
-       (as_seq h0 coins) (as_matrix h0 sp_matrix) (as_seq h0 d) (as_seq h0 ct))
+       (as_seq h0 coins) (as_matrix h0 sp_matrix) (as_seq h0 d))
 let crypto_kem_enc_ct_inner seed_a seed_e b coins sp_matrix d ct =
   let h0 = ST.get () in
   Spec.Frodo.KEM.expand_crypto_ciphertextbytes ();
@@ -301,7 +301,7 @@ let crypto_kem_enc_ct_inner seed_a seed_e b coins sp_matrix d ct =
   let h3 = ST.get () in
   LSeq.eq_intro (LSeq.sub #_ #(v crypto_ciphertextbytes) (as_seq h3 ct) (v c1Len) (v c2Len)) (as_seq h2 c2);
   LSeq.eq_intro (LSeq.sub #_ #(v crypto_ciphertextbytes) (as_seq h3 ct) 0 (v c1Len)) (as_seq h1 c1);
-  S.lemma_update_ct (as_seq h3 c1) (as_seq h3 c2) (as_seq h0 d) (as_seq h0 ct) (as_seq h3 ct)
+  S.lemma_update_ct (as_seq h3 c1) (as_seq h3 c2) (as_seq h0 d) (as_seq h3 ct)
 
 val crypto_kem_enc_ct:
     pk:lbytes crypto_publickeybytes
@@ -313,7 +313,7 @@ val crypto_kem_enc_ct:
       live h pk /\ live h g /\ live h coins /\ live h ct /\
       disjoint g ct /\ disjoint ct pk /\ disjoint coins ct)
     (ensures fun h0 _ h1 -> modifies (loc_buffer ct) h0 h1 /\
-      as_seq h1 ct == S.crypto_kem_enc_ct (as_seq h0 pk) (as_seq h0 g) (as_seq h0 coins) (as_seq h0 ct))
+      as_seq h1 ct == S.crypto_kem_enc_ct (as_seq h0 pk) (as_seq h0 g) (as_seq h0 coins))
 [@"c_inline"]
 let crypto_kem_enc_ct pk g coins ct =
   assert (v params_nbar * v params_n % 2 = 0);
@@ -341,15 +341,14 @@ val crypto_kem_enc_ss:
     (ensures  fun h0 _ h1 -> modifies (loc_buffer ss) h0 h1 /\
      (let c12 = LSeq.sub #_ #(v crypto_ciphertextbytes) (as_seq h0 ct) 0 (v crypto_ciphertextbytes - v crypto_bytes) in
       let kd = LSeq.sub #_ #(3 * v crypto_bytes) (as_seq h0 g) (v crypto_bytes) (2 * v crypto_bytes) in
-      as_seq h1 ss == S.update_ss c12 kd (as_seq h0 ss)))
+      as_seq h1 ss == S.update_ss c12 kd))
 [@"c_inline"]
 let crypto_kem_enc_ss g ct ss =
   push_frame();
   let ss_init_len = crypto_ciphertextbytes +! crypto_bytes in
   let ss_init:lbytes ss_init_len = create ss_init_len (u8 0) in
-  let kd = sub #uint8 #_ #(2 * v crypto_bytes) g crypto_bytes (size 2 *! crypto_bytes) in
-
   let c12 = sub ct (size 0) (crypto_ciphertextbytes -! crypto_bytes) in
+  let kd = sub #uint8 #_ #(2 * v crypto_bytes) g crypto_bytes (size 2 *! crypto_bytes) in
   let h0 = ST.get () in
   update_sub ss_init (size 0) (crypto_ciphertextbytes -! crypto_bytes) c12;
   update_sub ss_init (crypto_ciphertextbytes -! crypto_bytes) (size 2 *! crypto_bytes) kd;
@@ -363,24 +362,24 @@ inline_for_extraction noextract
 val crypto_kem_enc_0:
     coins:lbytes (params_nbar *! params_nbar *! params_extracted_bits /. size 8)
   -> pk:lbytes crypto_publickeybytes
-  -> pk_coins:lbytes (crypto_publickeybytes +! params_nbar *! params_nbar *! params_extracted_bits /. size 8)
   -> g:lbytes (size 3 *! crypto_bytes)
   -> Stack unit
     (requires fun h ->
-      live h coins /\ live h pk /\ live h pk_coins /\ live h g /\
-      disjoint pk_coins pk /\ disjoint pk_coins coins /\
-      disjoint pk_coins g)
-    (ensures  fun h0 _ h1 -> modifies (loc_union (loc_buffer pk_coins) (loc_buffer g)) h0 h1 /\
-      as_seq h1 g == S.crypto_kem_enc_0 (as_seq h0 coins) (as_seq h0 pk) (as_seq h0 pk_coins))
-let crypto_kem_enc_0 coins pk pk_coins g =
+      live h coins /\ live h pk /\ live h g)
+    (ensures  fun h0 _ h1 -> modifies (loc_buffer g) h0 h1 /\
+      as_seq h1 g == S.crypto_kem_enc_0 (as_seq h0 coins) (as_seq h0 pk))
+let crypto_kem_enc_0 coins pk g =
   let bytes_mu = params_nbar *! params_nbar *! params_extracted_bits /. size 8 in
+  push_frame();
+  let pk_coins:lbytes (crypto_publickeybytes +! bytes_mu) = create (crypto_publickeybytes +! bytes_mu) (u8 0) in
   let h0 = ST.get () in
   update_sub pk_coins (size 0) crypto_publickeybytes pk;
   update_sub pk_coins crypto_publickeybytes bytes_mu coins;
   let h2 = ST.get () in
   LSeq.eq_intro (LSeq.sub #_ #(v crypto_publickeybytes + v bytes_mu) (as_seq h2 pk_coins) 0 (v crypto_publickeybytes)) (as_seq h0 pk);
 
-  cshake_frodo (crypto_publickeybytes +! bytes_mu) pk_coins (u16 3) (size 3 *! crypto_bytes) g
+  cshake_frodo (crypto_publickeybytes +! bytes_mu) pk_coins (u16 3) (size 3 *! crypto_bytes) g;
+  pop_frame()
 
 inline_for_extraction noextract
 val crypto_kem_enc_1:
@@ -397,7 +396,7 @@ val crypto_kem_enc_1:
       disjoint g ss /\ disjoint g coins /\ disjoint g pk)
     (ensures  fun h0 _ h1 ->
       modifies (loc_union (loc_union (loc_buffer ct) (loc_buffer ss)) (loc_buffer g)) h0 h1 /\
-      (let ct_s, ss_s = S.crypto_kem_enc_1 (as_seq h0 g) (as_seq h0 coins) (as_seq h0 ct) (as_seq h0 ss) (as_seq h0 pk) in
+      (let ct_s, ss_s = S.crypto_kem_enc_1 (as_seq h0 g) (as_seq h0 coins) (as_seq h0 pk) in
       as_seq h1 ct == ct_s /\ as_seq h1 ss == ss_s))
 let crypto_kem_enc_1 g coins ct ss pk =
   assert_norm (2 * v crypto_bytes % 4 = 0);
@@ -417,23 +416,15 @@ val crypto_kem_enc_:
       disjoint ct ss /\ disjoint ct pk /\ disjoint ss pk /\
       disjoint coins ss /\ disjoint coins ct /\ disjoint coins pk)
     (ensures  fun h0 _ h1 -> modifies (loc_union (loc_buffer ct) (loc_buffer ss)) h0 h1 /\
-      (let ct_s, ss_s = S.crypto_kem_enc (as_seq h0 coins) (as_seq h0 pk) (as_seq h0 ct) (as_seq h0 ss) in
+      (let ct_s, ss_s = S.crypto_kem_enc (as_seq h0 coins) (as_seq h0 pk) in
       as_seq h1 ct == ct_s /\ as_seq h1 ss == ss_s))
 let crypto_kem_enc_ coins ct ss pk =
   push_frame();
   let bytes_mu = params_nbar *! params_nbar *! params_extracted_bits /. size 8 in
-  let pk_coins:lbytes (crypto_publickeybytes +! bytes_mu) = create (crypto_publickeybytes +! bytes_mu) (u8 0) in
   let g:lbytes (size 3 *! crypto_bytes) = create (size 3 *! crypto_bytes) (u8 0) in
-
-  let h0 = ST.get () in
-  crypto_kem_enc_0 coins pk pk_coins g;
-  let h1 = ST.get () in
-  assert (as_seq h1 g == S.crypto_kem_enc_0 (as_seq h0 coins) (as_seq h0 pk) (as_seq h0 pk_coins));
+  
+  crypto_kem_enc_0 coins pk g;
   crypto_kem_enc_1 g coins ct ss pk;
-  let h2 = ST.get () in
-  assert
-    (let ct_s, ss_s = S.crypto_kem_enc_1 (as_seq h1 g) (as_seq h0 coins) (as_seq h0 ct) (as_seq h0 ss) (as_seq h0 pk) in
-     as_seq h2 ct == ct_s /\ as_seq h2 ss == ss_s);
   pop_frame()
 
 inline_for_extraction noextract
